coq_session/proc_type.v
@@ -1,6 +1,6 @@
-From mathcomp Require Import ssreflect ssrbool eqtype ssrnat seq.
+From mathcomp Require Import ssreflect ssrbool eqtype ssrnat seq zify.
 From Coq Require Import ssrfun Classical Utf8.
-Require Export AutosubstSsr ARS proc_step dyn_cren.
+Require Export AutosubstSsr ARS proc_ast dyn_cren.
 
 Set Implicit Arguments.
 Unset Strict Implicit.
@@ -23,58 +23,80 @@ Inductive proc_type : dyn_ctx -> proc -> Prop :=
   Θ ⊢ ν.p
 where "Θ ⊢ p" := (proc_type Θ p).
 
-Lemma proc_congr0_sym p q : proc_congr0 p q -> proc_congr0 q p.
-Proof. elim; move=>*; eauto using proc_congr0. Qed.
+Inductive proc_wf : dyn_ctx -> Prop :=
+| proc_wf_nil : proc_wf nil
+| proc_wf_ty Θ r A :
+  proc_wf Θ ->
+  nil ⊢ A : Proto ->
+  proc_wf (Ch r A :L Θ)
+| proc_wf_n Θ :
+  proc_wf Θ ->
+  proc_wf (_: Θ).
 
-Lemma proc_crename Θ Θ' p ξ :
-  Θ ⊢ p -> dyn_ctx_cren ξ Θ Θ' -> Θ' ⊢ proc_cren p ξ.
+Lemma dyn_empty_proc_wf Θ : dyn_empty Θ -> proc_wf Θ.
+Proof with eauto using proc_wf. elim... Qed.
+
+Lemma dyn_just_proc_wf Θ x r A :
+  dyn_just Θ x (Ch r A) -> nil ⊢ A : Proto -> proc_wf Θ.
 Proof with eauto.
-  move=>ty. elim: ty Θ' ξ=>{Θ p}.
-  { move=>Θ m tym Θ' ξ agr/=.
-    constructor.
-    replace (IO Unit) with (term_cren (IO Unit) ξ) by eauto.
-    apply: dyn_crename.
-    apply: tym.
+  move e:(Ch r A)=>B js. elim: js r A e=>{Θ x B}.
+  { move=>Θ A emp r A0 e tyA0. destruct A; inv e.
+    have/={}tyA0:=sta_crename tyA0 (sta_agree_cren_nil (subn^~ 1)).
+    rewrite<-term_cren_comp in tyA0.
+    have e: ((+1) >>> (subn^~ 1)) = id.
+    { f_ext. move=>x. simpl. lia. }
+    rewrite e in tyA0.
+    rewrite term_cren_id in tyA0.
+    constructor...
+    apply: dyn_empty_proc_wf... }
+  { move=>Θ A x js ih r A0 e tyA0. destruct A; inv e.
+    have/={}tyA0:=sta_crename tyA0 (sta_agree_cren_nil (subn^~ 1)).
+    rewrite<-term_cren_comp in tyA0.
+    have e: ((+1) >>> (subn^~ 1)) = id.
+    { f_ext. move=>x0. simpl. lia. }
+    rewrite e in tyA0.
+    rewrite term_cren_id in tyA0.
     constructor... }
-  { move=>Θ1 Θ2 Θ p q mrg typ ihp tyq ihq Θ' ξ agr/=.
-    have[Θ1'[Θ2'[mrg'[agr1 agr2]]]]:=dyn_ctx_cren_merge agr mrg.
-    econstructor... }
-  { move=>Θ p r1 r2 A xor typ ihp Θ' ξ agr/=.
-    econstructor...
-    apply: ihp.
-    have tyA:nil ⊢ A : Proto by admit.
-    have tyA':nil ⊢ term_cren A (+1) : Proto by admit.
-    have agr0:=dyn_ctx_cren_ty r2 tyA agr.
-    have{}agr0:=dyn_ctx_cren_ty r1 tyA' agr0.
-    rewrite<-term_cren_comp in agr0.
-    have e:((+1) >>> upren ξ) = (ξ >>> (+1)) by autosubst.
-    rewrite e in agr0.
-    have{}e:(term_cren A (ξ >>> (+1)))= term_cren (term_cren A ξ) (+1).
-    by rewrite<-term_cren_comp.
-    rewrite e in agr0.
-    apply: agr0. }
-  {
-  }
+Qed.
 
-Lemma proc_congr0_type Θ p q : Θ ⊢ p -> proc_congr0 p q -> Θ ⊢ q.
-Proof with eauto using proc_type, proc_congr0.
-  move=>ty. elim: ty q=>{Θ p}.
-  { move=>Θ m tym q cgr. inv cgr. }
-  { move=>Θ1 Θ2 Θ p q mrg typ ihp tyq ihq q0 cgr. inv cgr.
-    { econstructor. apply: merge_sym. all: eauto. }
-    { inv tyq.
-      have[Θ4[mrg1 mrg2]]:=merge_splitL (merge_sym mrg) H1.
-      econstructor. apply: mrg2.
-      econstructor. apply: merge_sym mrg1.
-      all: eauto. }
-    { admit. }
-    { admit. }
-    { admit. }
-    { admit. } }
-  { move=>Θ p r1 r2 A d typ ihp q cgr. inv cgr.
-    { inv typ. inv H1; inv H5.
-      { econstructor. apply: H2.
-        econstructor...
-      }
-    }
-  }
+Lemma proc_wf_merge Θ1 Θ2 Θ :
+  Θ1 ∘ Θ2 => Θ -> proc_wf Θ1 -> proc_wf Θ2 -> proc_wf Θ.
+Proof with eauto using proc_wf.
+  elim=>{Θ1 Θ2 Θ}...
+  { move=>Θ1 Θ2 Θ m mrg ih wf1 wf2. inv wf1. }
+  { move=>Θ1 Θ2 Θ m mrg ih wf1 wf2. inv wf1. inv wf2... }
+  { move=>Θ1 Θ2 Θ m mrg ih wf1 wf2. inv wf1. inv wf2... }
+  { move=>Θ1 Θ2 Θ mrg ih wf1 wf2. inv wf1. inv wf2... }
+Qed.
+
+Lemma dyn_type_proc_wf Θ Γ Δ m A : Θ ; Γ ; Δ ⊢ m : A -> proc_wf Θ.
+Proof with eauto using proc_wf.
+  elim=>{Θ Γ Δ m A}...
+  { move=>Θ Γ Δ x s A emp wf shs dhs. apply: dyn_empty_proc_wf... }
+  { move=>Θ1 Θ2 Θ Γ Δ1 Δ2 Δ A B m n s mrg1 mrg2 tym ihm tyn ihn.
+    apply: proc_wf_merge mrg1 ihm ihn. }
+  { move=>Θ1 Θ2 Θ Γ Δ1 Δ2 Δ A B m n t mrg1 mrg2 tyS tym ihm tyn ihn.
+    apply: proc_wf_merge mrg1 ihm ihn. }
+  { move=>Θ1 Θ2 Θ Γ Δ1 Δ2 Δ A B C m n s r t mrg1 mrg2 tyC tym ihm tyn ihn.
+    apply: proc_wf_merge mrg1 ihm ihn. }
+  { move=>Θ1 Θ2 Θ Γ Δ1 Δ2 Δ A B C m n s r1 r2 t mrg1 mrg2 tyC tym ihm tyn ihn.
+    apply: proc_wf_merge mrg1 ihm ihn. }
+  { move=>Θ Γ Δ emp wf k. apply: dyn_empty_proc_wf... }
+  { move=>Θ Γ Δ emp wf k. apply: dyn_empty_proc_wf... }
+  { move=>Θ Γ Δ emp wf k. apply: dyn_empty_proc_wf... }
+  { move=>Θ1 Θ2 Θ Γ Δ1 Δ2 Δ A m n1 n2 s mrg1 mrg2
+           tyA tym ihm tyn1 ihn1 tyn2 ihn2.
+    apply: proc_wf_merge mrg1 ihm ihn1. }
+  { move=>Θ1 Θ2 Θ Γ Δ1 Δ2 Δ m n A B s t mrg1 mrg2 tyB tym ihm tyn ihn.
+    apply: proc_wf_merge mrg1 ihm ihn. }
+  { move=>Θ Γ Δ r x A js wf k tyA.
+    apply: dyn_just_proc_wf... }
+Qed.
+
+Lemma proc_type_wf Θ p : Θ ⊢ p -> proc_wf Θ.
+Proof with eauto using proc_wf.
+  elim=>{Θ p}.
+  { move=>Θ m tym. apply: dyn_type_proc_wf... }
+  { move=>Θ1 Θ2 Θ p q mrg typ ihp tyq ihq. apply: proc_wf_merge... }
+  { move=>Θ p r1 r2 A e typ wf. inv wf. inv H1... }
+Qed.
