coq_session/proc_sr.v
@@ -1,0 +1,56 @@
+From mathcomp Require Import ssreflect ssrbool eqtype ssrnat seq.
+From Coq Require Import ssrfun Classical Utf8.
+Require Export AutosubstSsr ARS proc_type proc_step.
+
+Set Implicit Arguments.
+Unset Strict Implicit.
+Unset Printing Implicit Defensive.
+
+Lemma proc_congr0_sym p q : proc_congr0 p q -> proc_congr0 q p.
+Proof. elim; move=>*; eauto using proc_congr0. Qed.
+
+Lemma proc_congr0_type Θ p q : Θ ⊢ p -> proc_congr0 p q -> Θ ⊢ q.
+Proof with eauto using proc_type, proc_congr0.
+  move=>ty. elim: ty q=>{Θ p}.
+  { move=>Θ m tym q cgr. inv cgr. }
+  { move=>Θ1 Θ2 Θ p q mrg typ ihp tyq ihq q0 cgr. inv cgr.
+    { econstructor. apply: merge_sym. all: eauto. }
+    { inv tyq.
+      have[Θ4[mrg1 mrg2]]:=merge_splitL (merge_sym mrg) H1.
+      econstructor. apply: mrg2.
+      econstructor. apply: merge_sym mrg1.
+      all: eauto. }
+    { inv typ.
+      have[Θ4[mrg1 mrg2]]:=merge_splitR mrg H1.
+      econstructor. apply: (merge_sym mrg2). apply: H3.
+      econstructor... }
+    { inv typ.
+      have wf:=proc_type_wf H2. inv wf. inv H1.
+      have mrg': 
+        Ch (~~r2) (term_cren A (+1)) :L Ch r2 A :L Θ1 ∘ _: _: Θ2 =>
+        Ch (~~r2) (term_cren A (+1)) :L Ch r2 A :L Θ.
+      repeat econstructor; eauto.
+      econstructor...
+      econstructor...
+      replace (proc_cren q (+2)) with (proc_cren (proc_cren q (+1)) (+1)).
+      apply: proc_cweaken.
+      apply: proc_cweaken...
+      rewrite<-proc_cren_comp.
+      by asimpl. }
+    { econstructor... }
+    { econstructor.
+      apply: mrg.
+      apply: ihp. apply: proc_congr0_sym...
+      apply: ihq. apply: proc_congr0_sym... } }
+  { move=>Θ p r1 r2 A d typ ihp q cgr. inv cgr.
+    { inv typ. inv H1; inv H5.
+      { econstructor. apply: H2.
+        econstructor...
+        apply: proc_cstrengthen.
+        apply: proc_cstrengthen.
+        rewrite<-proc_cren_comp.
+        by asimpl. }
+      {
+      }
+    }
+  }
